updates

interp_test/add.v
@@ -11,32 +11,41 @@
 
 *)
 
+(* required because the libraries ITree + CertiCoq break together *)
 Unset Universe Checking.
-From Wasm Require Import datatypes prettyprint.
 
-From CertiCoq Require Import LambdaANF.toplevel Common.Common Common.compM Common.Pipeline_utils.
-Require Import ExtLib.Structures.Monad.
-From MetaCoq.Template Require Import bytestring MCString.
+
+(* From CertiCoq Require Import Common.Common Common.compM Common.Pipeline_utils. *)
+
+(* From MetaCoq.Utils Require Import bytestring MCString. *)
 From Coq Require Import ZArith List.
 
-From CertiCoq Require Import LambdaANF.cps LambdaANF.cps_show CodegenWASM.wasm_map_util CodegenWASM.LambdaANF_to_WASM.
+(* From CertiCoq Require Import LambdaANF.cps LambdaANF.cps_show CodegenWASM.LambdaANF_to_WASM. *)
+Require Import ExtLib.Structures.Monad.
 Import MonadNotation.
 
 From Coq.Strings Require Import Byte.
 
 From Wasm Require Import binary_format_parser binary_format_printer host
-                         datatypes_properties check_toks instantiation.
+                         datatypes datatypes_properties check_toks instantiation_func interpreter_itree.
 
+From mathcomp Require Import seq.
+
+
+Check ([:: 1; 2]). (* WasmCert uses the ssreflect package a lot, these  *)
+(* fails: Check ([1;2]). *)
+Import ListNotations.
+Check [1;2].
 
 
 Module TestModule.
 
+(* python script in certicoqwasm-testing turns .wasm in list of bytes one can copy paste here *)
 Definition test_bytes : list Byte.byte := x00 :: x61 :: x73 :: x6d :: x01 :: x00 :: x00 :: x00 :: x01 :: x07 :: x01 :: x60 :: x02 :: x7f :: x7f :: x01 :: x7f :: x03 :: x02 :: x01 :: x00 :: x07 :: x0b :: x01 :: x07 :: x61 :: x64 :: x64 :: x5f :: x69 :: x33 :: x32 :: x00 :: x00 :: x0a :: x09 :: x01 :: x07 :: x00 :: x20 :: x00 :: x20 :: x01 :: x6a :: x0b :: nil.
 
 Definition test_module_opt : option module := run_parse_module test_bytes.
 Compute test_module_opt.
 
-From mathcomp Require Import seq.
 
 Definition test_module := {|
   mod_types := [:: Tf [:: T_i32; T_i32] [:: T_i32]];
@@ -62,20 +71,19 @@ Definition test_module := {|
         |}]
 |}.
 
-
 Definition type_check_test_module :=
   m <- test_module_opt ;;
   module_type_checker m.
 
 Compute type_check_test_module.
 
-Definition test_function_type := Tf [T_i32; T_i32] [T_i32].
+Definition test_function_type := Tf [:: T_i32; T_i32] [:: T_i32].
 Definition test_function := {|
                 modfunc_type := Mk_typeidx 0;
-                modfunc_locals := [T_i32];
+                modfunc_locals := [:: T_i32];
                 modfunc_body :=
-                  [BI_get_local 0; BI_get_local 1;
-                  BI_binop T_i32 (Binop_i BOI_add)]
+                  [:: BI_get_local 0; BI_get_local 1;
+                      BI_binop T_i32 (Binop_i BOI_add)]
               |}.
 
 End TestModule.
@@ -84,553 +92,132 @@ End TestModule.
 Definition nat_to_i32 (n : nat) :=
   VAL_int32 (Wasm_int.Int32.repr (BinInt.Z.of_nat n)).
 
-Import TestModule.
+(* Import TestModule. *)
 From mathcomp Require Import eqtype.
-From Wasm Require Import host opsem instantiation.
+From Wasm Require Import host opsem instantiation_func.
 
 Section OpsemTest.
-Require Import Lia.
+Import Lia.
 Import Relations.Relation_Operators.
 
-From Wasm Require Import interpreter_sound.
+Import interpreter_func.
 
-From mathcomp Require Import ssreflect ssrfun ssrnat ssrbool eqtype seq.
-From StrongInduction Require Import StrongInduction Inductions.
+Import ssreflect ssrfun ssrnat ssrbool eqtype seq.
 
 Set Implicit Arguments.
 Unset Strict Implicit.
 Unset Printing Implicit Defensive.
 
-
-From Wasm Require Export operations opsem interpreter_func interpreter_func_sound properties common.
+Import operations opsem interpreter_itree interpreter_func properties common.
 
 Variable host_function : eqType.
 Let store_record := store_record host_function.
-Let function_closure := function_closure host_function.
-(*Let administrative_instruction := administrative_instruction host_function.
-
-Let to_e_list : seq basic_instruction -> seq administrative_instruction := @to_e_list _.
-Let to_b_list : seq administrative_instruction -> seq basic_instruction := @to_b_list _.*)
-Let e_typing : store_record -> t_context -> seq administrative_instruction -> function_type -> Prop :=
-  @e_typing _.
-Let inst_typing : store_record -> instance -> t_context -> bool := @inst_typing _.
-(*Let reduce_simple : seq administrative_instruction -> seq administrative_instruction -> Prop :=
-  @reduce_simple _.
-Let const_list : seq administrative_instruction -> bool := @const_list _.
-Let lholed := lholed host_function.
-Let lfilled : depth -> lholed -> seq administrative_instruction -> seq administrative_instruction -> bool :=
-  @lfilled _.
-Let lfilledInd : depth -> lholed -> seq administrative_instruction -> seq administrative_instruction -> Prop :=
-  @lfilledInd _.
-Let es_is_basic : seq administrative_instruction -> Prop := @es_is_basic _.*)
-
 Let host := host host_function.
-
-(*Let run_one_step_fuel := @run_one_step_fuel host_function.*)
-
-Let RS_crash := interpreter_func.RS_crash.
-Let RS_break := interpreter_func.RS_break.
-Let RS_return := interpreter_func.RS_return.
-Let RS_normal := interpreter_func.RS_normal.
-
 Variable host_instance : host.
-
-Let run_step_fuel := @run_step_fuel host_function host_instance.
-
 Let host_state := host_state host_instance.
 
-Let reduce : host_state -> store_record -> frame -> seq administrative_instruction ->
-             host_state -> store_record -> frame -> seq administrative_instruction -> Prop
-  := @reduce _ _.
+Let reduce_trans := @reduce_trans host_function host_instance.
 
-Variable host_application_impl : host_state -> store_record -> function_type -> host_function -> seq value ->
-                       (host_state * option (store_record * result)).
-
-Hypothesis host_application_impl_correct :
-  (forall hs s ft hf vs hs' hres, (host_application_impl hs s ft hf vs = (hs', hres)) -> host_application hs s ft hf vs hs' hres).
-
-Let run_one_step := @run_one_step host_function host_instance host_application_impl.
-Let run_step := @run_step host_function host_instance host_application_impl.
-Let run_step_with_fuel := @run_step_with_fuel host_function host_instance host_application_impl.
+Definition initial_store : store_record := {|
+  (* imported funcs write_int and write_char, they are not called
+     but need to be present:
+     s_funcs := [FC_func_host (Tf [T_i32] []) host_function; FC_func_host (Tf [T_i32] []) host_function];
+     *)
+    s_funcs := nil;
+    s_tables := nil;
+    s_mems := nil;
+    s_globals := nil;
+  |}.
 
 (** The lemmas [r_eliml] and [r_elimr] are the fundamental framing lemmas.
   They enable to focus on parts of the stack, ignoring the context. **)
 
-(** The following tactics are meant to help the proof of [run_step_soundness] below. **)
-(** Simplify an hypothesis, possibly rewriting it everywhere. **)
-Ltac simplify_hypothesis Hb :=
-  repeat rewrite length_is_size in Hb;
-  repeat match type of Hb with
-  | is_true (es_is_trap _) => move/es_is_trapP: Hb => Hb
-  | is_true (const_list (_ :: _)) => rewrite const_list_cons in Hb
-  | ?b = true => fold (is_true b) in Hb
-  | (_ == _) = false => move/eqP in Hb
-  | context C [size (rev _)] => rewrite size_rev in Hb
-  | context C [take _ (rev _)] => rewrite take_rev in Hb
-  | context C [rev (rev _)] => rewrite revK in Hb
-  | context C [true && _] => rewrite Bool.andb_true_l in Hb
-  | context C [_ && true] => rewrite Bool.andb_true_r in Hb
-  | context C [false || _] => rewrite Bool.orb_false_l in Hb
-  | context C [_ || false] => rewrite Bool.orb_false_r in Hb
-  | is_true true => clear Hb
-  | is_true false => exfalso; apply: notF; apply: Hb
-  | is_true (_ == _) => move/eqP in Hb
-  | ?x = ?x => clear Hb
-  | _ = _ => rewrite Hb in *
-  end.
+Lemma r_eliml: forall hs s f es hs' s' f' es' lconst,
+  const_list lconst ->
+  reduce (host_instance := host_instance) hs s f es hs' s' f' es' ->
+  reduce hs s f (lconst ++ es) hs' s' f' (lconst ++ es').
+Proof.
+  move => hs s f es hs' s' f' es' lconst HConst H.
+  apply: r_label; try apply/lfilledP.
+  - by apply: H.
+  - replace (lconst++es) with (lconst++es++[::]); first by apply: LfilledBase.
+    f_equal. by apply: cats0.
+  - replace (lconst++es') with (lconst++es'++[::]); first by apply: LfilledBase.
+    f_equal. by apply: cats0.
+Qed.
 
-(** Apply [simplify_hypothesis] to all hypotheses. **)
-Ltac simplify_goal :=
-  repeat match goal with H: _ |- _ => progress simplify_hypothesis H end.
+Lemma r_elimr: forall hs s f es hs' s' f' es' les,
+    reduce (host_instance := host_instance) hs s f es hs' s' f' es' ->
+    reduce hs s f (es ++ les) hs' s' f' (es' ++ les).
+Proof.
+  move => hs s f es hs' s' f' es' les H.
+  apply: r_label; try apply/lfilledP.
+  - apply: H.
+  - replace (es++les) with ([::]++es++les) => //. by apply: LfilledBase.
+  - replace (es'++les) with ([::]++es'++les) => //. by apply: LfilledBase.
+Qed.
 
-(** A common pattern in the proof: using an hypothesis on the form [rev l = l'] to rewrite [l]. **)
-Ltac subst_rev_const_list :=
- repeat lazymatch goal with
- | HRevConst: rev ?lconst = ?h :: ?t |- _ =>
-   apply rev_move in HRevConst; rewrite HRevConst; rewrite -cat1s; rewrite rev_cat;
-   rewrite -v_to_e_cat; rewrite -catA
- end.
-
-(** Simplify the lists in the goal. **)
-Ltac simplify_lists :=
-  (** Common rewriting rules. **)
-  repeat first [
-      rewrite drop_rev
-    | rewrite take_rev
-    | rewrite revK
-    | rewrite length_is_size
-    | rewrite size_take
-    | rewrite size_drop
-    | rewrite size_rev
-    | rewrite v_to_e_size
-    | rewrite rev_cat
-    | rewrite rev_cons -cats1
-    | rewrite -v_to_e_cat
-    | rewrite -v_to_e_rev
-    | rewrite -v_to_e_take
-    | rewrite -v_to_e_drop];
-  (** Putting all the lists into a normal form, as concatenations of as many things.
-    Because [cat1s] conflicts with [cats0], replacing any occurence of [[X]] to
-    [[X] ++ [::]], it has to be done separately.
-    Rewrite with the associated [math goal with] is avoid to deal with existential
-    vairables. **)
+Ltac separate_instr :=
+  cbn;
   repeat match goal with
   |- context C [?x :: ?l] =>
      lazymatch l with [::] => fail | _ => rewrite -(cat1s x l) end
-  end;
-  repeat lazymatch goal with
-  | |- context C [[::] ++ _] => rewrite cat0s
-  | |- context C [_ ++ [::]] => rewrite cats0
-  | |- context C [rcons _ _] => rewrite -cats1
-  | |- context C [(_ ++ _) ++ _] => rewrite -catA
-  | |- context C [rev [::]] => rewrite rev0
-  | |- context C [v_to_e_list [::]] => rewrite v_to_e_list0
-  | |- context C [v_to_e_list [:: _]] => rewrite v_to_e_list1
-  end;
-  try subst_rev_const_list.
-
-(** Explode a tuple into all its components. **)
-Ltac explode_value v :=
-  lazymatch type of v with
-  | (_ * _)%type =>
-    let v1 := fresh "v1" in
-    let v2 := fresh "v2" in
-    destruct v as [v1 v2];
-    explode_value v1;
-    explode_value v2
-  | _ => idtac
   end.
 
-(** Try to find which variable to pattern match on, destruct it,
-  then simplify the destructing equality. **)
-Ltac explode_and_simplify :=
-  repeat lazymatch goal with
-  | |- ?T = _ -> _ =>
-    lazymatch T with
-    | context C [split_n ?l ?n] => rewrite (split_n_is_take_drop l n)
-    | context C [vs_to_es ?l] => rewrite/vs_to_es
-    | context C [host_application_impl _ _ _ _ _ _] =>
-      destruct host_application_impl
-    | context C [match ?b with true => ?v1 | false => ?v2 end] =>
-      let Hb := fresh "if_expr" in
-      destruct b eqn:Hb;
-      simplify_hypothesis Hb;
-      try by [|apply: Hb]
-    | context C [match rev ?lconst with
-                 | _ :: _ => _
-                 | _ => _
-                 end] =>
-      let HRevConst := fresh "HRevConst" in
-      destruct (rev lconst) eqn:HRevConst;
-      simplify_hypothesis HRevConst;
-      try by [|apply: HRevConst]
-    | context C [match ?v with
-                 | VAL_int32 _ => _
-                 | _ => _
-                 end] =>
-      let Hb := fresh "Ev" in
-      destruct v eqn:Hb;
-      simplify_hypothesis Hb;
-      try by []
-    | context C [match ?v with
-                 | Some _ => _
-                 | _ => _
-                 end] =>
-      let Hv := fresh "option_expr" in
-      let v' := fresh "v" in
-      destruct v as [v'|] eqn:Hv; [ explode_value v' |];
-      simplify_hypothesis Hv;
-      try by [|apply: Hv]
-    | context C [match ?cl with
-                 | FC_func_native _ _ _ _ => _
-                 | FC_func_host _ _ => _
-                 end] =>
-      let Hcl := fresh "Hcl" in
-      destruct cl eqn:Hcl;
-      simplify_hypothesis Hcl;
-      try by []
-    | context C [match ?tf with
-                 | Tf _ _ => _
-                 end] =>
-      let Hcl := fresh "Htf" in
-      destruct tf eqn:Htf;
-      simplify_hypothesis Htf;
-      try by []
-    | context C [match ?v with
-                 | T_i32 => _
-                 | T_i64 => _
-                 | T_f32 => _
-                 | T_f64 => _
-                 end] =>
-      let Hv := fresh "Ev" in
-      destruct v eqn:Hv;
-      simplify_hypothesis Hv;
-      try by []
-    | context C [match ?v with
-                 | CVO_convert => _
-                 | CVO_reinterpret => _
-                 end] =>
-      let Hv := fresh "Ecvtop" in
-      destruct v eqn:Hv;
-      simplify_hypothesis Hv;
-      try by []
-    | context C [match ?v with
-                 | Tf _ _ => _
-                 end] =>
-      let vs1 := fresh "vs" in
-      let vs2 := fresh "vs" in
-      let Hv := fresh "Eft" in
-      destruct v as [vs1 vs2] eqn:Hv;
-      simplify_hypothesis Hv;
-      try by []
-    | context C [expect ?X ?f ?err] =>
-       let HExpect := fresh "HExpect" in
-       destruct X eqn:HExpect;
-       simplify_hypothesis HExpect;
-       simpl;
-       try by [|apply: HExpect]
-    | context C [match ?l with
-                 | _ :: _ => _
-                 | _ => _
-                 end] =>
-      destruct l;
-      try by []
-    end
-  end;
-  simplify_lists.
-
-(** If the goal is on the form [c1 = c2 -> property] where [c1] and [c2] are two configurations,
-  then invert it. **)
-Ltac pattern_match :=
-  let go _ :=
-    lazymatch goal with
-    | |- (_, _, _, _) = (_, _, _, _) -> _ =>
-      let H := fresh in
-      move=> H; inversion H; subst; clear H
-    end in
-  go tt || (simpl; go tt).
-
-(** Eliminate the stack frame, by applying [r_elimr] and [r_eliml] according to some heuristics. **)
-Ltac stack_frame :=
-  repeat lazymatch goal with
-  | |- reduce _ _ _ (_ :: ?l) _ _ _ _ =>
-    rewrite -cat1s
-  | |- reduce _ _ _ (?l1 ++ ?l2 :: ?l3) _ _ _ ((?l5 ++ ?l4) ++ ?l3) =>
-    rewrite -cat1s; rewrite catA;
-    apply: r_elimr; try apply: r_eliml; try apply: v_to_e_is_const_list
-  | |- reduce _ _ _ (?l1 ++ ?l2 :: ?l3) _ _ _ (?l5 ++ ?l3) =>
-    rewrite -cat1s; rewrite catA;
-    apply: r_elimr; try apply: r_eliml_empty; try apply: v_to_e_is_const_list
-  | |- reduce _ _ _ (operations.v_to_e_list ?l1 ++ _) _ _ _ (operations.v_to_e_list (take ?n ?l1) ++ _) =>
-    rewrite (v_to_e_take_drop_split l1 n); rewrite -catA;
-    apply: r_eliml; try apply: v_to_e_is_const_list
+(* applies r_elimr with es := (the first n const ++ the following instruction)
+   the remaining ones are put in les *)
+Ltac elimr_nary_instr n :=
+  let H := fresh "H" in
+  match n with
+  | 0 => lazymatch goal with
+         | |- reduce _ _ _ ([:: ?instr] ++ ?l3) _ _ _ ?l4 => apply r_elimr
+          end
+  | 1 => lazymatch goal with
+         | |- reduce _ _ _ ([::AI_basic (BI_const ?c1)] ++
+                            [::AI_basic ?instr] ++ ?l3) _ _ _ ?l4 =>
+            assert ([:: AI_basic (BI_const c1)] ++ [:: AI_basic instr] ++ l3
+                  = [:: AI_basic (BI_const c1);
+                        AI_basic instr] ++ l3) as H by reflexivity; rewrite H; apply r_elimr; clear H
+          end
+  | 2 => lazymatch goal with
+         | |- reduce _ _ _ ([::AI_basic (BI_const ?c1)] ++
+                            [::AI_basic (BI_const ?c2)] ++
+                            [::AI_basic ?instr] ++ ?l3) _ _ _ ?l4 =>
+            assert ([:: AI_basic (BI_const c1)] ++ [:: AI_basic (BI_const c2)] ++ [:: AI_basic instr] ++ l3
+                  = [:: AI_basic (BI_const c1);
+                        AI_basic (BI_const c2);
+                        AI_basic instr] ++ l3) as H by reflexivity; rewrite H; apply r_elimr; clear H
+          end
   end.
 
-(** Try to solve a goal of the form [const_list _]. **)
-Ltac solve_const_list :=
-  repeat rewrite const_list_concat;
-  repeat rewrite const_list_cons;
-  by [| apply: v_to_e_is_const_list ].
+Ltac dostep :=
+  eapply rt_trans with (y := (?[hs], ?[sr], ?[f'], ?[s] ++ ?[t])); first apply rt_step; separate_instr.
 
-(** Try to solve a goal of the form [l1 = l2] where [l1] and [l2] are two lists. **)
-Ltac show_list_equality :=
-  simplify_lists; simplify_goal;
-  by [| repeat f_equal
-      | repeat rewrite catA; repeat f_equal
-      | repeat rewrite -catA; repeat f_equal
-      | eauto
-      | erewrite cats0; eauto
-      | erewrite cat0s; eauto
-      | repeat (repeat rewrite catA; f_equal; repeat rewrite -catA; f_equal)
-      | repeat (repeat rewrite -catA; f_equal; repeat rewrite catA; f_equal) ].
+(* only returns single list of instructions *)
+Ltac dostep' :=
+   eapply rt_trans with (y := (?[hs], ?[sr], ?[f'], ?[s])); first  apply rt_step; separate_instr.
 
-(** Given a left and a right frame, rewrite the goal to move these frames out. **)
-Ltac frame_out l r :=
-  lazymatch goal with
-  | |- reduce _ _ _ ?st1 _ _ _ ?st2 =>
-    let sta := fresh "st1" in
-    evar (sta : seq administrative_instruction);
-    let stb := fresh "st2" in
-    evar (stb : seq administrative_instruction);
-    let Est1 := fresh "E_before" in
-    assert (Est1: st1 = (l ++ sta) ++ r); [
-        rewrite/sta {sta stb}; try show_list_equality
-      | let Est2 := fresh "E_after" in
-        assert (Est2: st2 = (l ++ stb) ++ r); [
-            rewrite/stb {Est1 sta stb}; try show_list_equality
-          | rewrite Est1 Est2;
-            apply r_elimr with (les := r);
-            apply r_eliml with (lconst := l); first try solve_const_list;
-            rewrite /sta /stb {Est1 Est2 sta stb};
-            try by repeat constructor ] ]
-  end.
-
-(** Same as [frame_out], by the frames are inferred (syntactically). **)
-Ltac auto_frame :=
-  simplify_lists;
-  let empty := constr:([::] : list administrative_instruction) in
-  let left _ :=
-    repeat rewrite -catA;
-    repeat lazymatch goal with
-    | |- reduce _ _ _ (?l ++ _) _ _ _ (?l ++ _) =>
-      frame_out l empty
-    | |- reduce _ _ _ (?l ++ _) _ _ _ ?l =>
-      frame_out l empty
-    | |- reduce _ _ _ ?l _ _ _ (?l ++ _) =>
-      frame_out l empty
-    end in
-  let right _ :=
-    repeat rewrite catA;
-    repeat lazymatch goal with
-    | |- reduce _ _ _ (_ ++ ?r) _ _ _ (_ ++ ?r) =>
-      frame_out empty r
-    | |- reduce _ _ _ (_ ++ ?r) _ _ _ ?r =>
-      frame_out empty r
-    | |- reduce _ _ _ ?r _ _ _ (_ ++ ?r) =>
-      frame_out empty r
-    end;
-    (** Renormalising back. **)
-    repeat (rewrite -catA) in
-  repeat first [ progress left tt | progress right tt ].
-
-(** Same as [frame_out], by the frames are existential variables. **)
-Ltac eframe :=
-  let l := fresh "l" in
-  evar (l : seq administrative_instruction);
-  let r := fresh "r" in
-  evar (r : seq administrative_instruction);
-  frame_out l r.
-
-(***********)
-
-From Wasm Require Import interpreter_func_sound.
+(********************************************************************************************)
 
 (* rt: rt_step, rt_refl, rt_trans *)
-Check instance.
-Print instance.
-Lemma test_reduces (inst : instance) (hs_initial : host_state)
-                   (hs_result : host_state) :
-  reduce_trans (hs_initial, empty_store_record host_function, Build_frame [nat_to_i32 1; nat_to_i32 2] inst , map AI_basic test_function.(modfunc_body))
-               (hs_initial, empty_store_record host_function, Build_frame [nat_to_i32 1; nat_to_i32 2] inst, [AI_basic (BI_const (nat_to_i32 3))]).
+Check clos_refl_trans. Print clos_refl_trans.
+
+(* frame, see datatypes.v *)
+Check frame. Print frame.
+
+Lemma test_reduces (hs : host_state) f :
+  f.(f_locs) = [nat_to_i32 1; nat_to_i32 2] ->
+  reduce_trans (hs, initial_store, f, [ AI_basic (BI_get_local 0); AI_basic (BI_get_local 1)
+                                      ; AI_basic (BI_binop T_i32 (Binop_i BOI_add))])
+               (hs, initial_store, f, [AI_basic (BI_const (nat_to_i32 3))]).
 Proof.
+  intro Hfr. cbn.
+  dostep. elimr_nary_instr 0. apply r_get_local. rewrite Hfr. reflexivity.
+  dostep. apply r_eliml. auto. elimr_nary_instr 0. apply r_get_local. rewrite Hfr. reflexivity.
   cbn.
-  eapply rt_trans with (y := (?[hs], ?[sr], ?[f], ?[s] ++ ?[t])).
-  {
-    apply rt_step. cbn.
-    explode_and_simplify.
-    replace ([:: AI_basic (BI_get_local 0); AI_basic (BI_get_local 1);
-        AI_basic (BI_binop T_i32 (Binop_i BOI_add))]) with
-        ([:: AI_basic (BI_get_local 0)] ++ ([AI_basic (BI_get_local 1);
-        AI_basic (BI_binop T_i32 (Binop_i BOI_add))])).
-    apply r_elimr. apply r_get_local. cbn. reflexivity.
-    reflexivity.
-  }
-  cbn.
-  eapply rt_trans with (y := (?[hs], ?[sr], ?[f], ?[s] ++ ?[t])).
-  {
-    eapply rt_step. cbn.
-    explode_and_simplify.
-    rewrite catA.
-    apply r_elimr.
-    apply r_eliml; auto.
-    apply r_get_local. reflexivity.
-  }
-  cbn. apply rt_step. cbn. apply r_simple. constructor. (* compute. *) reflexivity.
+  (* dostep. apply r_simple. apply rs_binop_success.
+  doesn't work here, unification error with anonymous var. *)
+  dostep'. apply r_simple. apply rs_binop_success. reflexivity.
+  apply rt_refl.
 Qed.
 End OpsemTest.
-
-From Wasm Require Import interpreter_func common operations opsem interpreter_func properties.
-
-From mathcomp Require Import seq.
-
-Section InterpTest.
-(* preamble pasted from interpreter_func_sound.v*)
-
-Variable host_function : eqType.
-Let store_record := store_record host_function.
-Let function_closure := function_closure host_function.
-(*Let administrative_instruction := administrative_instruction host_function.
-
-Let to_e_list : seq basic_instruction -> seq administrative_instruction := @to_e_list _.
-Let to_b_list : seq administrative_instruction -> seq basic_instruction := @to_b_list _.*)
-Let e_typing : store_record -> t_context -> seq administrative_instruction -> function_type -> Prop :=
-  @e_typing _.
-Let inst_typing : store_record -> instance -> t_context -> bool := @inst_typing _.
-(*Let reduce_simple : seq administrative_instruction -> seq administrative_instruction -> Prop :=
-  @reduce_simple _.
-Let const_list : seq administrative_instruction -> bool := @const_list _.
-Let lholed := lholed host_function.
-Let lfilled : depth -> lholed -> seq administrative_instruction -> seq administrative_instruction -> bool :=
-  @lfilled _.
-Let lfilledInd : depth -> lholed -> seq administrative_instruction -> seq administrative_instruction -> Prop :=
-  @lfilledInd _.
-Let es_is_basic : seq administrative_instruction -> Prop := @es_is_basic _.*)
-
-Let host := host host_function.
-
-(*Let run_one_step_fuel := @run_one_step_fuel host_function.*)
-
-Let RS_crash := interpreter_func.RS_crash.
-Let RS_break := interpreter_func.RS_break.
-Let RS_return := interpreter_func.RS_return.
-Let RS_normal := interpreter_func.RS_normal.
-
-Variable host_instance : host.
-
-Let run_step_fuel := @run_step_fuel host_function host_instance.
-
-Let host_state := host_state host_instance.
-
-Let reduce : host_state -> store_record -> frame -> seq administrative_instruction ->
-             host_state -> store_record -> frame -> seq administrative_instruction -> Prop
-  := @reduce _ _.
-
-Variable host_application_impl : host_state -> store_record -> function_type -> host_function -> seq value ->
-                       (host_state * option (store_record * result)).
-
-Hypothesis host_application_impl_correct :
-  (forall hs s ft hf vs hs' hres, (host_application_impl hs s ft hf vs = (hs', hres)) -> host_application hs s ft hf vs hs' hres).
-
-
-Let run_one_step := @run_one_step host_function host_instance host_application_impl.
-Let run_step := @run_step host_function host_instance host_application_impl.
-Let run_step_with_fuel := @run_step_with_fuel host_function host_instance host_application_impl.
-Let run_v := @run_v host_function host_instance host_application_impl.
-
-(* Fixpoint run_v (fuel : fuel) (d : depth) (cfg : config_tuple) : ((host_state * store_record * res)%type) := *)
-
-Definition test_run (inst : instance) (hs_initial : host_state) :=
-  run_v 10 5 (hs_initial, empty_store_record host_function, Build_frame [nat_to_i32 0] inst,
-               map AI_basic [ BI_const (nat_to_i32 2)
-                            ; BI_const (nat_to_i32 3)
-                            ; BI_set_local 0
-                            ; BI_get_local 0
-                            ; BI_binop T_i32 (Binop_i BOI_add)
-                            ]).
-
-Compute test_run.
-
-Lemma test_run_correct (inst : instance) (hs_initial : host_state) :
-  let '(_, _, res) := test_run inst hs_initial in
-  res = R_value [nat_to_i32 5].
-Proof.
-  vm_compute. reflexivity.
-Qed.
-End InterpTest.
-
-(*
-Section OpsemTest.
-(* preamble pasted from interpreter_func_sound.v*)
-
-Variable host_function : eqType.
-Let store_record := store_record host_function.
-Let function_closure := function_closure host_function.
-(*Let administrative_instruction := administrative_instruction host_function.
-
-Let to_e_list : seq basic_instruction -> seq administrative_instruction := @to_e_list _.
-Let to_b_list : seq administrative_instruction -> seq basic_instruction := @to_b_list _.*)
-Let e_typing : store_record -> t_context -> seq administrative_instruction -> function_type -> Prop :=
-  @e_typing _.
-Let inst_typing : store_record -> instance -> t_context -> bool := @inst_typing _.
-
-Let host := host host_function.
-
-(*Let run_one_step_fuel := @run_one_step_fuel host_function.*)
-
-Let RS_crash := interpreter_func.RS_crash.
-Let RS_break := interpreter_func.RS_break.
-Let RS_return := interpreter_func.RS_return.
-Let RS_normal := interpreter_func.RS_normal.
-
-Variable host_instance : host.
-
-Let run_step_fuel := @run_step_fuel host_function host_instance.
-
-Let host_state := host_state host_instance.
-
-Let reduce : host_state -> store_record -> frame -> seq administrative_instruction ->
-             host_state -> store_record -> frame -> seq administrative_instruction -> Prop
-  := @reduce _ _.
-
-Variable host_application_impl : host_state -> store_record -> function_type -> host_function -> seq value ->
-                       (host_state * option (store_record * result)).
-
-Hypothesis host_application_impl_correct :
-  (forall hs s ft hf vs hs' hres, (host_application_impl hs s ft hf vs = (hs', hres)) -> host_application hs s ft hf vs hs' hres).
-
-
-Let run_one_step := @run_one_step host_function host_instance host_application_impl.
-Let run_step := @run_step host_function host_instance host_application_impl.
-Let run_step_with_fuel := @run_step_with_fuel host_function host_instance host_application_impl.
-Let run_v := @run_v host_function host_instance host_application_impl.
-
-
-Let executable_host := executable_host host_function.
-
-Import Monads.
-Import MonadNotation.
-
-From Coq Require Import String.
-From Wasm Require Import interpreter.
-From mathcomp Require Import seq.
-
-Import TestModule.
-
-Unset Universe Checking.
-
-Check lookup_exported_function.
-
-Check name.
-Print name.
-
-Check eqtype.Equality.type.
-
-Print interp_instantiate_wrapper.
-Definition to_seq {A} (l : list A) : seq A := l.
-
-Definition run :=
-  interp_instantiate_wrapper host_function test_module.
-  Some instantiated_module.
-  (* cfg_tuple <- lookup_exported_function (to_seq (list_byte_of_string "add_i32")) instantiated_module;;*)
-  Some 1.
-*)
